Define type pbit for readable adequacy lemmas.

theories/program_logic/adequacy.v
@@ -35,24 +35,24 @@ Proof.
 Qed.
 
 (* Program logic adequacy *)
-Record adequate {Λ} (p : bool) (e1 : expr Λ) (σ1 : state Λ) (φ : val Λ → Prop) := {
+Record adequate {Λ} (p : pbit) (e1 : expr Λ) (σ1 : state Λ) (φ : val Λ → Prop) := {
   adequate_result t2 σ2 v2 :
    rtc step ([e1], σ1) (of_val v2 :: t2, σ2) → φ v2;
   adequate_safe t2 σ2 e2 :
-   p →
+   p = progress →
    rtc step ([e1], σ1) (t2, σ2) →
-   e2 ∈ t2 → progress e2 σ2
+   e2 ∈ t2 → language.progress e2 σ2
 }.
 
 Theorem adequate_tp_safe {Λ} (e1 : expr Λ) t2 σ1 σ2 φ :
-  adequate true e1 σ1 φ →
+  adequate progress e1 σ1 φ →
   rtc step ([e1], σ1) (t2, σ2) →
   Forall (λ e, is_Some (to_val e)) t2 ∨ ∃ t3 σ3, step (t2, σ2) (t3, σ3).
 Proof.
   intros Had ?.
   destruct (decide (Forall (λ e, is_Some (to_val e)) t2)) as [|Ht2]; [by left|].
   apply (not_Forall_Exists _), Exists_exists in Ht2; destruct Ht2 as (e2&?&He2).
-  destruct (adequate_safe true e1 σ1 φ Had t2 σ2 e2) as [?|(e3&σ3&efs&?)];
+  destruct (adequate_safe progress e1 σ1 φ Had t2 σ2 e2) as [?|(e3&σ3&efs&?)];
     rewrite ?eq_None_not_Some; auto.
   { exfalso. eauto. }
   destruct (elem_of_list_split t2 e2) as (t2'&t2''&->); auto.
@@ -60,7 +60,7 @@ Proof.
 Qed.
 
 Section adequacy.
-Context `{irisG Λ Σ} (p : bool).
+Context `{irisG Λ Σ} (p : pbit).
 Implicit Types e : expr Λ.
 Implicit Types P Q : iProp Σ.
 Implicit Types Φ : val Λ → iProp Σ.
@@ -136,9 +136,9 @@ Proof.
 Qed.
 
 Lemma wp_safe E e σ Φ :
-  world' E σ ∗ wp' E e Φ ==∗ ▷ ⌜if p then progress e σ else True⌝.
+  world' E σ ∗ wp' E e Φ ==∗ ▷ ⌜if p then language.progress e σ else True⌝.
 Proof.
-  rewrite wp_unfold /wp_pre /progress. iIntros "[(Hw&HE&Hσ) [H|[_ H]]]".
+  rewrite wp_unfold /wp_pre /language.progress. iIntros "[(Hw&HE&Hσ) [H|[_ H]]]".
   { iDestruct "H" as (v) "[% _]"; destruct p; eauto 10. }
   rewrite fupd_eq. iMod ("H" with "* Hσ [-]") as ">(?&?&%&?)"; first by iFrame.
   destruct p; eauto 10.
@@ -147,7 +147,7 @@ Qed.
 Lemma wptp_safe n e1 e2 t1 t2 σ1 σ2 Φ :
   nsteps step n (e1 :: t1, σ1) (t2, σ2) → e2 ∈ t2 →
   world σ1 ∗ wp e1 Φ ∗ wptp t1 ⊢
-  Nat.iter (S (S n)) (λ P, |==> ▷ P) ⌜if p then progress e2 σ2 else True⌝.
+  Nat.iter (S (S n)) (λ P, |==> ▷ P) ⌜if p then language.progress e2 σ2 else True⌝.
 Proof.
   intros ? He2. rewrite wptp_steps //; rewrite (Nat_iter_S_r (S n)). apply bupd_iter_mono.
   iDestruct 1 as (e2' t2') "(% & Hw & H & Htp)"; simplify_eq.
@@ -189,7 +189,7 @@ Proof.
     rewrite Nat_iter_S. iMod wsat_alloc as (Hinv) "[Hw HE]".
     rewrite fupd_eq in Hwp; iMod (Hwp with "[$Hw $HE]") as ">(Hw & HE & Hwp)".
     iDestruct "Hwp" as (Istate) "[HI Hwp]".
-    iModIntro. iNext. iApply (@wptp_safe _ _ (IrisG _ _ Hinv Istate) true); eauto.
+    iModIntro. iNext. iApply (@wptp_safe _ _ (IrisG _ _ Hinv Istate) progress); eauto.
     iFrame. by iApply big_sepL_nil.
 Qed.
 
