theories/heap_lang/adequacy.v
@@ -15,7 +15,7 @@ Proof. intros [? ?]%subG_inv; split; apply _. Qed.
 
 Definition heap_adequacy Σ `{heapPreG Σ} e σ φ :
   (∀ `{heapG Σ}, True ⊢ WP e {{ v, ⌜φ v⌝ }}) →
-  adequate true e σ φ.
+  adequate progress e σ φ.
 Proof.
   intros Hwp; eapply (wp_adequacy _ _); iIntros (?) "".
   iMod (own_alloc (● to_gen_heap σ)) as (γ) "Hh".
